examples/low-level/rst.fst
@@ -6,8 +6,8 @@
 
 module RST
 
-open FStar.Set
-open FStar.List
+(** This module defines the [RST] effect of computations that occur within our
+    stack of regions. *)
 
 open Located
 open Regions
@@ -16,80 +16,82 @@ open Lref
 kind Pre  = smem -> Type
 kind Post (a:Type) = a -> smem -> Type
 
+new_effect StSTATE = STATE_h smem
 
-new_effect StSTATE = STATE_h smem //TODO: move this to sst.fst
 effect RST (a:Type) (pre:Pre) (post: (smem -> Post a)) =
-        StSTATE a
-              (fun (p:Post a) (h:smem) -> pre h /\ (forall a h1. (pre h  /\ post h a h1) ==> p a h1)) (* WP *)
-              (fun (p:Post a) (h:smem) -> (forall a h1. (pre h  /\ post h a h1) ==> p a h1))          (* WLP *)
+  StSTATE a
+    (fun (p:Post a) (h:smem) -> pre h /\ (forall a h1. (pre h /\ post h a h1) ==> p a h1)) (* WP *)
+    (fun (p:Post a) (h:smem) -> (forall a h1. (pre h /\ post h a h1) ==> p a h1)) (* WLP *)
 
-assume val halloc:  #a:Type -> init:a -> RST (lref a)
-                                         (fun m -> True)
-                                         (fun m0 r m1 -> allocateInBlock r (hp m0)  (hp m1) init /\ (snd m0 = snd m1) /\ refLoc r == InHeap)
 
-assume val salloc:  #a:Type -> init:a -> RST (lref a)
-     (fun m -> b2t (Stack.isNonEmpty (st m))) (*why is "== true" required here, but not at other places? : *)
-     (*Does F* have (user defined?) implicit coercions? : Not yet *)
+(** Operations for allocation, reading and writing into our new (axiomatized)
+    memory. The functions below are axiomatized, because when extracting to
+    OCaml code, we replace them with calls to our custom memory allocator. *)
+
+(* Allocate in the garbage-collected heap. This is the [ref] ML function. *)
+assume val halloc: #a:Type -> init:a ->
+  RST (lref a)
+    (fun m -> True)
+    (fun m0 r m1 -> allocatedInRegion r (hp m0) (hp m1) init /\ (snd m0 = snd m1) /\ refLoc r == InHeap)
+
+(* Allocate in the top-most region. This is a new, [ref]-like function. *)
+assume val ralloc:  #a:Type -> init:a -> RST (lref a)
+     mStackNonEmpty
      (fun m0 r m1 ->
-          (Stack.isNonEmpty (st m0)) /\ (Stack.isNonEmpty (st m1))
-          /\ allocateInBlock r (topRegion m0) (topRegion m1) init
-          /\ refLoc r = InStack (topRegionId m0) /\ (topRegionId m0 = topRegionId m1)
+          Stack.isNonEmpty (st m0) /\ Stack.isNonEmpty (st m1)
+          /\ allocatedInRegion r (topRegion m0) (topRegion m1) init
+          /\ refLoc r = InStack (topRegionId m0) /\ topRegionId m0 = topRegionId m1
           /\ Regions.tail m0 = Regions.tail m1 /\ m1 = allocateInTopR r init m0)
 
-assume val memread:  #a:Type -> r:(lref a) -> RST a
-	  (fun m -> b2t (liveRef r m))
-    (fun m0 a m1 -> m0=m1 /\ (liveRef r m0) /\ lookupRef r m0 = a)
 
-assume val memwrite:  #a:Type -> r:(lref a) -> v:a ->
+(* Read from the top-most region. This is the [!] ML operator. *)
+assume val memread:  #a:Type -> r:lref a ->
+  RST a
+    (fun m -> b2t (liveRef r m))
+    (fun m0 a m1 -> m0=m1 /\ liveRef r m0 /\ lookupRef r m0 = a)
+
+(* Write in the top-most region. This is the [:=] ML operator. *)
+assume val memwrite:  #a:Type -> r:lref a -> v:a ->
   RST unit
-	    (fun m -> b2t (liveRef r m))
-      (fun m0 _ m1 -> (liveRef r m1)
-        /\ (writeMemAux r m0 v) =  m1)
+    (fun m -> b2t (liveRef r m))
+    (fun m0 _ m1 -> liveRef r m1
+               /\ writeMemAux r m0 v =  m1)
 
-(*
-Free can only deallocate a heap-allocated lref. The implementation
-below doesn't make sense becasue it allows even deallocation of stack
-references
 
-assume val freeRef:  #a:Type -> r:(lref a)  ->
-  RST unit
-	    (fun m -> b2t (liveRef r m))
-      (fun m0 _ m1 -> (freeMemAux r m0) ==  m1)
-*)
-
-(*make sure that the ids are monotone *)
-assume val pushStackFrame:  unit -> RST unit
+(** Two operations for manipulating the stack of regions. *)
+assume val pushRegion:  unit -> RST unit
     (fun m -> True)
     (fun m0 _ m1 ->
-             (Regions.tail m1 = m0)
-          /\ (Stack.isNonEmpty (st m1))
+             Regions.tail m1 = m0
+          /\ Stack.isNonEmpty (st m1)
           /\ topRegion m1 = emp)
 
-assume val popStackFrame:  unit -> RST unit
-    (fun m -> b2t (Stack.isNonEmpty (st m)))
-    (fun m0 _ m1 -> Regions.tail m0 ==  m1)
+assume val popRegion:  unit -> RST unit
+    mStackNonEmpty
+    (fun m0 _ m1 -> Regions.tail m0 == m1)
 
 
-(** Injection of DIV effect into the new effect, mostly copied from prims.fst*)
+(** Injection of the [DIV] effect into the [RST] effect, mostly copied from prims.fst *)
 kind RSTPost (a:Type) = STPost_h smem a
-
 
 sub_effect
   DIV  ~> StSTATE = fun (a:Type) (wp:PureWP a) (p : RSTPost a) (h:smem)
                 -> wp (fun a -> p a h)
 
+(** Some effect abbreviations. *)
 
+(* Effect of a computation that leaves the region stack's structure unchanged
+   (i.e. no push or pop) but may 
 effect Mem (a:Type) (pre: smem -> Type) (post: (smem -> RSTPost a)) (mod: modset) =
         RST a pre (fun m0 a m1 -> post m0 a m1 /\ rids m0 = rids m1 /\ canModify m0 m1 mod)
 
 //TODO: MemReader?
-effect PureMem (a:Type) (pre:smem -> Type) (post: ( smem -> a -> Type)) =
+effect PureMem (a:Type) (pre:smem -> Type) (post: smem -> a -> Type) =
         RST a pre (fun m0 a m1 -> post m1 a /\ m0=m1)
 
-open FStar.Ghost
-assume val get : unit -> PureMem (erased smem)
+assume val get : unit -> PureMem (FStar.Ghost.erased smem)
       (requires (fun m -> true))
-      (ensures (fun m v -> reveal v = m))
+      (ensures (fun m v -> FStar.Ghost.reveal v = m))
 
 (*
  * In future, we would like to enforce that the type a is locatable and immutable.
@@ -97,7 +99,7 @@ assume val get : unit -> PureMem (erased smem)
  * When allocating mutable things, the ghost memory of RST must be updated to
  * keep track of its "current" value. Because lalloc is a PureMem, it cannot be used.
  * PureMem means lalloc does not change smem, the map from references to their values.
- * For refs, use instead salloc above. for arrays, use [hs]create in array.fsi instead.
+ * For refs, use instead ralloc above. for arrays, use [hs]create in array.fsi instead.
  *)
  (*is this is ever renamed or moved, mlp_lalloc in src\extraction\ml-syntax.fs MUST be updated.*)
  (*as of now, a can only be a record type.*)
@@ -105,7 +107,7 @@ assume val get : unit -> PureMem (erased smem)
 Extraction will then avoid creating this value on the heap.*)
 assume val lalloc: #a:Type -> v:a -> PureMem
   (located a)
-  (requires (fun m ->Stack.isNonEmpty (st m)))
+  (requires mStackNonEmpty)
   (ensures (fun m1 l -> lreveal l = v /\ Stack.isNonEmpty (st m1) /\ regionOf l = InStack (topRegionId m1)))
 
 //TODO: This is not sound; take f as the identity function
@@ -123,4 +125,16 @@ assume val llift : #a:Type -> #b:Type -> f:(components a b) -> l:located a
               (ensures (fun v m1 -> v == f (greveal l) ))
 
 
+*)
+
+
+(*
+Free can only deallocate a heap-allocated lref. The implementation
+below doesn't make sense becasue it allows even deallocation of stack
+references
+
+assume val freeRef:  #a:Type -> r:(lref a)  ->
+  RST unit
+	    (fun m -> b2t (liveRef r m))
+      (fun m0 _ m1 -> (freeMemAux r m0) ==  m1)
 *)
